New resolver passes

Source/DafnyCore/AST/Expressions/Heap/FieldReferrer.cs
@@ -4,7 +4,7 @@
 /// The right-hand-side of an expression of the type obj`fieldName
 /// Denotes the memory location at this index
 /// </summary>
-public class FieldReferrer: Expression, ICloneable<FieldReferrer> {
+public class FieldLocation: Expression, ICloneable<FieldLocation> {
   // Because memory locations are tuples, this is just a copy of the expression so that we can determine if
   // it's legit to 
   public Expression ObjectCopy { get; }
@@ -13,17 +13,17 @@ public class FieldReferrer: Expression, ICloneable<FieldReferrer> {
   [FilledInDuringResolution]
   public Field ResolvedField { get; set; }
   
-  public FieldReferrer(Expression objectCopy, Name name) : base(name.Origin) {
+  public FieldLocation(Expression objectCopy, Name name) : base(name.Origin) {
     this.ObjectCopy = objectCopy;
     this.Name = name;
   }
 
-  public FieldReferrer(Cloner cloner, FieldReferrer original) : base(cloner, original) {
+  public FieldLocation(Cloner cloner, FieldLocation original) : base(cloner, original) {
     this.ObjectCopy = cloner.CloneExpr(original.ObjectCopy);
     this.Name = original.Name;
   }
 
-  public FieldReferrer Clone(Cloner cloner) {
-    return new FieldReferrer(cloner, this);
+  public FieldLocation Clone(Cloner cloner) {
+    return new FieldLocation(cloner, this);
   }
 }
